rupicola/stlc/Examples.fst
@@ -1,16 +1,28 @@
 module Examples
 
+open QTyp
+
+let ut_unit = ()
+let ut_true = true
+let ut_false = false
+
+val var0 : fs_oexp (extend qBool empty) qBool
+let var0 fsG = hd fsG
+
+val var1 : fs_oexp (extend qBool (extend qBool empty)) qBool
+let var1 fsG = hd (tail fsG)
+
+let var2 : fs_oexp (extend qBool (extend qBool (extend qBool empty))) qBool =
+  fun fsG -> hd (tail (tail fsG))
+
+let constant (x: bool) : bool =
+  true
+
 let identity : bool -> bool =
   fun x -> x
 
 let thunked_id : bool -> bool -> bool =
   fun x y -> y
-
-let call_arg : (unit -> unit) -> unit =
-  fun f -> f ()
-
-let call_arg2 : (bool -> bool -> bool) -> bool =
-  fun f -> f true false
 
 let proj1 : bool -> bool -> bool -> bool =
   fun x y z -> x
@@ -20,6 +32,24 @@ let proj2 : bool -> bool -> bool -> bool =
 
 let proj3 : bool -> bool -> bool -> bool =
   fun x y z -> z
+
+let apply_top_level_def : bool -> bool =
+  fun x -> thunked_id x true
+
+let apply_top_level_def' : bool -> bool -> bool =
+  fun x y -> thunked_id x y
+
+let papply__top_level_def : bool -> bool -> bool =
+  fun x -> thunked_id x
+
+let apply_arg : (unit -> unit) -> unit =
+  fun f -> f ()
+
+let apply_arg2 : (bool -> bool -> bool) -> bool =
+  fun f -> f true false
+
+let papply_arg2 : (bool -> bool -> bool) -> bool -> bool =
+  fun f -> f true
 
 let anif : bool = if true then false else true
 
@@ -37,3 +67,20 @@ let callback_return : bool -> (bool -> bool) =
 
 let callback_return' : bool -> (bool -> bool) =
   fun x -> if x then (fun _ -> x) else identity
+
+let make_pair : bool -> bool -> (bool & bool) =
+  fun x y -> (x, y)
+
+let pair_of_functions : (bool -> bool) & (bool -> bool -> bool) =
+  (fun x -> negb x), (fun x y -> y)
+
+let pair_of_functions2 : (bool -> bool) & (bool -> bool -> bool) =
+  (negb, if2)
+
+let fst_pair : bool = fst (true, ())
+let wrap_fst : (bool & bool) -> bool = fun p -> fst p
+let wrap_fst_pa : (bool & bool) -> bool = fst
+
+let snd_pair : unit = snd (true, ())
+let wrap_snd : (bool & unit) -> unit = fun p -> snd p
+let wrap_snd_pa : (bool & unit) -> unit = snd
