rupicola/stlc/QExp.fst
@@ -1,5 +1,6 @@
 module QExp
 
+open FStar.Tactics
 open QTyp
 
 (** These helper functions are necessary to help F* do unification
@@ -31,14 +32,6 @@ val helper_unit : g:typ_env -> fs_oexp g qUnit
 let helper_unit g _ = ()
 
 unfold
-val helper_true : g:typ_env -> fs_oexp g qBool
-let helper_true g _ = true
-
-unfold
-val helper_false : g:typ_env -> fs_oexp g qBool
-let helper_false g _ = false
-
-unfold
 val helper_app: #g : typ_env ->
                 #a : qType ->
                 #b : qType ->
@@ -48,16 +41,6 @@ val helper_app: #g : typ_env ->
 let helper_app f x fsG = (f fsG) (x fsG)
 
 unfold
-val helper_if : #g :typ_env ->
-                #a  : qType ->
-                c   : fs_oexp g qBool ->
-                t   : fs_oexp g a ->
-                e   : fs_oexp g a ->
-                fs_oexp g a
-let helper_if c t e fsG =
-    if c fsG then t fsG else e fsG
-
-unfold
 val helper_lambda : #g :typ_env ->
                 #a :qType ->
                 #b :qType ->
@@ -65,12 +48,54 @@ val helper_lambda : #g :typ_env ->
                 fs_oexp (extend a g) b
 let helper_lambda #_ #_ f fsG = f (tail fsG) (hd fsG)
 
+unfold
+val helper_true : g:typ_env -> fs_oexp g qBool
+let helper_true g _ = true
+
+unfold
+val helper_false : g:typ_env -> fs_oexp g qBool
+let helper_false g _ = false
+
+unfold
+val helper_if : #g :typ_env ->
+                #a  : qType ->
+                c   : fs_oexp g qBool ->
+                t   : fs_oexp g a ->
+                e   : fs_oexp g a ->
+                fs_oexp g a
+let helper_if c t e fsG =
+  if c fsG then t fsG else e fsG
+
+unfold
+val helper_pair : #g : typ_env ->
+                  #a : qType ->
+                  #b : qType ->
+                  x : fs_oexp g a ->
+                  y : fs_oexp g b ->
+                  fs_oexp g (a ^* b)
+let helper_pair #_ #_ #_ x y fsG =
+  (x fsG, y fsG)
+
+unfold
+val helper_fst : #g : typ_env ->
+                 #a : qType ->
+                 #b : qType ->
+                 p : fs_oexp g (a ^* b) ->
+                 fs_oexp g a
+let helper_fst #_ #_ #_ p fsG = fst (p fsG)
+
+unfold
+val helper_snd : #g : typ_env ->
+                 #a : qType ->
+                 #b : qType ->
+                 p : fs_oexp g (a ^* b) ->
+                 fs_oexp g b
+let helper_snd #_ #_ #_ p fsG = snd (p fsG)
+
 [@@no_auto_projectors] // FStarLang/FStar#3986
 noeq
 type exp_quotation : #a:qType -> g:typ_env -> fs_oexp g a -> Type =
 | Qtt         : #g : typ_env -> exp_quotation g (helper_unit g)
-| QTrue       : #g : typ_env -> exp_quotation g (helper_true g)
-| QFalse      : #g : typ_env -> exp_quotation g (helper_false g)
 
 | QVar0       : #g : typ_env ->
                 #a : qType ->
@@ -96,6 +121,15 @@ type exp_quotation : #a:qType -> g:typ_env -> fs_oexp g a -> Type =
                 exp_quotation g x ->
                 exp_quotation g (helper_app #_ #_ #_ f x)
 
+| QLambda     : #g : typ_env ->
+                #a : qType ->
+                #b : qType ->
+                #f : fs_oexp g (a ^-> b) ->
+                exp_quotation (extend a g) (helper_lambda f) ->
+                exp_quotation g f
+
+| QTrue       : #g : typ_env -> exp_quotation g (helper_true g)
+| QFalse      : #g : typ_env -> exp_quotation g (helper_false g)
 | QIf         : #g : typ_env ->
                 #a : qType ->
                 #c : fs_oexp g qBool ->
@@ -106,12 +140,26 @@ type exp_quotation : #a:qType -> g:typ_env -> fs_oexp g a -> Type =
                 exp_quotation g e ->
                 exp_quotation g (helper_if c t e)
 
-| QLambda     : #g : typ_env ->
-                #a : qType ->
-                #b : qType ->
-                #f : fs_oexp g (a ^-> b) ->
-                exp_quotation (extend a g) (helper_lambda f) ->
-                exp_quotation g f
+| QMkpair   : #g : typ_env ->
+              #a : qType ->
+              #b : qType ->
+              #x : fs_oexp g a ->
+              #y : fs_oexp g b ->
+              exp_quotation g x ->
+              exp_quotation g y ->
+              exp_quotation g (helper_pair x y)
+| QFst      : #g : typ_env ->
+              #a : qType ->
+              #b : qType ->
+              #p : fs_oexp g (a ^* b) ->
+              exp_quotation g p ->
+              exp_quotation g (helper_fst p)
+| QSnd      : #g : typ_env ->
+              #a : qType ->
+              #b : qType ->
+              #p : fs_oexp g (a ^* b) ->
+              exp_quotation g p ->
+              exp_quotation g (helper_snd p)
 
 unfold
 let helper_oexp (#a:qType) (x:get_Type a) : fs_oexp empty a = fun _ -> x
@@ -123,6 +171,34 @@ open Examples
 
 #push-options "--no_smt"
 
+let test_ut_unit
+  : closed_exp_quotation qUnit ut_unit
+  = Qtt
+
+let test_ut_true
+  : closed_exp_quotation qBool ut_true
+  = QTrue
+
+let test_ut_false
+  : closed_exp_quotation qBool ut_false
+  = QFalse
+
+let test_var0
+  : exp_quotation #qBool (extend qBool empty) var0
+  = QVar0
+
+let test_var1
+  : exp_quotation #qBool (extend qBool (extend qBool empty)) var1
+  = QVar1
+
+let test_var2
+  : exp_quotation #qBool (extend qBool (extend qBool (extend qBool empty))) var2
+  = QVar2
+
+let test_constant
+  : closed_exp_quotation (qBool ^-> qBool) constant
+  = QLambda QTrue
+
 let test_identity
   : closed_exp_quotation (qBool ^-> qBool) identity
   = QLambda QVar0
@@ -130,14 +206,6 @@ let test_identity
 let test_thunked_id
   : closed_exp_quotation (qBool ^-> (qBool ^-> qBool)) thunked_id
   = QLambda (QLambda QVar0)
-
-let test_call_arg
-  : closed_exp_quotation ((qUnit ^-> qUnit) ^-> qUnit) call_arg
-  = QLambda (QApp QVar0 Qtt)
-
-let test_call_arg2
-  : closed_exp_quotation ((qBool ^-> qBool ^-> qBool) ^-> qBool) call_arg2
-  = QLambda (QApp (QApp QVar0 QTrue) QFalse)
 
 let test_proj1
   : closed_exp_quotation (qBool ^-> qBool ^-> qBool ^-> qBool) proj1
@@ -150,6 +218,37 @@ let test_proj2
 let test_proj3
   : closed_exp_quotation (qBool ^-> qBool ^-> qBool ^-> qBool) proj3
   = QLambda (QLambda (QLambda QVar0))
+
+let test_apply_top_level_def
+  : closed_exp_quotation (qBool ^-> qBool) apply_top_level_def
+  = QLambda (QApp
+              (QApp #_ #_ #_ #(fun _ x y -> y) // TODO: why cannot it infer this? is it difficult to unfold thunked_id?
+                (QLambda (QLambda QVar0))
+                QVar0)
+              QTrue)
+
+let test_apply_top_level_def'
+  : closed_exp_quotation (qBool ^-> qBool ^-> qBool) apply_top_level_def'
+  = QLambda (QLambda (QApp
+                      (QApp #_ #_ #_ #(fun _ x y -> y)
+                        (QLambda (QLambda QVar0))
+                        QVar1)
+                      QVar0))
+
+let test_papply__top_level_def
+  : closed_exp_quotation (qBool ^-> qBool ^-> qBool) papply__top_level_def
+  = QLambda (QApp #_ #_ #_ #(fun _ x y -> y)
+              (QLambda (QLambda QVar0))
+              QVar0)
+
+let test_apply_arg
+  : closed_exp_quotation ((qUnit ^-> qUnit) ^-> qUnit) apply_arg
+  = QLambda (QApp QVar0 Qtt)
+
+let test_apply_arg2
+  : closed_exp_quotation ((qBool ^-> qBool ^-> qBool) ^-> qBool) apply_arg2
+  = QLambda (QApp (QApp QVar0 QTrue) QFalse)
+
 
 [@expect_failure]
 let test_proj2'
@@ -164,22 +263,20 @@ let test_negb
   : closed_exp_quotation (qBool ^-> qBool) negb
   = QLambda (QIf QVar0 QFalse QTrue)
 
-let test_if2
-  : closed_exp_quotation (qBool ^-> qBool ^-> qBool) if2
-  = QLambda (QLambda (QIf QVar1 QFalse QVar0))
-
 let test_negb_pred
   : closed_exp_quotation ((qBool ^-> qBool) ^-> qBool ^-> qBool) negb_pred
   = QLambda (QLambda (QIf (QApp QVar1 QVar0) QFalse QTrue))
 
-open FStar.Tactics
+let test_if2
+  : closed_exp_quotation (qBool ^-> qBool ^-> qBool) if2
+  = QLambda (QLambda (QIf QVar1 QFalse QVar0))
 
 (** Because of the fancy types, now one needs a preprocessing tactic to
     get rid of the qTypes **)
 
 let simplify_qType (x:term) : Tac term =
   (** TODO: why is F* not doing this automatically anyway? **)
-  norm_term_env (top_env ()) [delta_only [`%qUnit; `%qBool; `%op_Hat_Subtraction_Greater; `%op_Hat_Star; `%get_rel; `%get_Type; `%Mkdtuple2?._1;`%Mkdtuple2?._2];iota] x
+  norm_term_env (top_env ()) [delta_only [`%fs_oexp; `%qUnit; `%qBool; `%op_Hat_Subtraction_Greater; `%op_Hat_Star; `%get_rel; `%get_Type; `%Mkdtuple2?._1;`%Mkdtuple2?._2];iota] x
 
 [@@ (preprocess_with simplify_qType)]
 let test_callback_return
@@ -195,14 +292,52 @@ let test_callback_return'
                        (QLambda #_ #_ #_ #(fun fsG y -> hd fsG) QVar1)
                        (QLambda #_ #_ #_ #(fun fsG -> identity) QVar0)) // TODO: why does it not work to unfold identity here?
 
-(**
-let project_equiv #g #a (qa:typ_quotation a) (s:fs_oexp g a) (qs:exp_quotation g s) :
-  Lemma (s `equiv qa` (project_exp q)) = ()
+let test_make_pair
+  : closed_exp_quotation (qBool ^-> qBool ^-> (qBool ^* qBool)) make_pair
+  = QLambda (QLambda (QMkpair QVar1 QVar0))
 
-  match qs with
-  | Qtt -> equiv_qUnit g
-  | QApp #_ #a #b #f qf #x qx ->
-      project_equiv (QArr ? qa) f qf;
-      project_equiv ? x qx;
-      equiv_app g ? qa f (project_exp f) x (project_exp x)
-**)
+// #set-options "--print_implicits"
+// [@@ (preprocess_with simplify_qType)]
+
+// TODO: why does this fail?
+let test_pair_of_functions
+  : closed_exp_quotation 
+    ((qBool ^-> qBool) ^* (qBool ^-> qBool ^-> qBool))
+    (FStar.Pervasives.norm [delta_only [`%pair_of_functions; `%negb]] pair_of_functions)
+  = admit (); QMkpair
+      (QLambda (QApp #_ #_ #_ #(fun _ x -> if x then false else true)
+                  (QLambda (QIf QVar0 QFalse QTrue))
+                  QVar0))
+      (QLambda (QLambda QVar0))
+
+let test_pair_of_functions2
+  : closed_exp_quotation 
+    ((qBool ^-> qBool) ^* (qBool ^-> qBool ^-> qBool))
+    (FStar.Pervasives.norm [delta_only [`%pair_of_functions2]] pair_of_functions2)
+  = admit (); QMkpair
+      (QLambda (QIf QVar0 QFalse QTrue))
+      (QLambda (QLambda (QIf QVar1 QFalse QVar0)))
+
+let test_fst_pair 
+  : closed_exp_quotation (qBool) fst_pair
+  = (QFst (QMkpair QTrue Qtt))
+
+let test_wrap_fst
+  : closed_exp_quotation ((qBool ^* qBool) ^-> qBool) wrap_fst
+  = QLambda (QFst QVar0)
+
+let test_wrap_fst_pa
+  : closed_exp_quotation ((qBool ^* qBool) ^-> qBool) wrap_fst_pa
+  = QLambda (QFst QVar0)
+
+let test_snd_pair 
+  : closed_exp_quotation (qUnit) snd_pair
+  = (QSnd (QMkpair QTrue Qtt))
+
+let test_wrap_snd
+  : closed_exp_quotation ((qBool ^* qUnit) ^-> qUnit) wrap_snd
+  = QLambda (QSnd QVar0)
+
+let test_wrap_snd_pa
+  : closed_exp_quotation ((qBool ^* qUnit) ^-> qUnit) wrap_snd_pa
+  = QLambda (QSnd QVar0)
