rupicola/stlc/Compilation.fst
@@ -10,14 +10,18 @@ open ExpRel
 let rec compile #g #a (#s:fs_oexp g a) (qs:exp_quotation g s) : Tot exp (decreases qs) =
   match qs with
   | Qtt -> EUnit
-  | QFalse -> EFalse
-  | QTrue -> ETrue
   | QVar0 -> EVar 0
   | QVar1 -> EVar 1
   | QVar2 -> EVar 2
   | QApp qf qx -> EApp (compile qf) (compile qx)
-  | QIf qc qt qe -> EIf (compile qc) (compile qt) (compile qe)
   | QLambda qbody -> ELam (compile qbody)
+  | QFalse -> EFalse
+  | QTrue -> ETrue
+  | QIf qc qt qe -> EIf (compile qc) (compile qt) (compile qe)
+  | QMkpair q1 q2 -> EPair (compile q1) (compile q2)
+  | QFst qp -> EFst (compile qp)
+  | QSnd qp -> ESnd (compile qp)
+
 
 let lem_compile_empty_closed #a (#s:fs_oexp empty a) (qs:exp_quotation empty s) : Lemma (is_closed (compile qs)) = admit ()
 
@@ -25,12 +29,10 @@ let compile_closed (#a:qType) (#s:get_Type a) (qs:exp_quotation #a empty (fun _ 
   lem_compile_empty_closed qs;
   compile qs
 
-let rec compile_equiv #g #a (#s:fs_oexp g a) (qs:exp_quotation g s)
+let rec compile_equiv #g (#a:qType) (#s:fs_oexp g a) (qs:exp_quotation g s)
   : Lemma (ensures (s `equiv a` (compile qs))) (decreases qs)
   = match qs with
   | Qtt -> equiv_unit g
-  | QFalse -> equiv_false g
-  | QTrue -> equiv_true g
   | QVar0 -> admit () // equiv_var g 0
   | QVar1 -> admit () // equiv_var g 1
   | QVar2 -> admit () //equiv_var g 2
@@ -38,11 +40,6 @@ let rec compile_equiv #g #a (#s:fs_oexp g a) (qs:exp_quotation g s)
     compile_equiv qf;
     compile_equiv qx;
     equiv_app f x (compile qf) (compile qx)
-  | QIf #_ #_ #c qc #t qt #e qe ->
-    compile_equiv qc;
-    compile_equiv qt;
-    compile_equiv qe;
-    equiv_if c t e (compile qc) (compile qt) (compile qe)
   | QLambda #_ #_ #_ #f qbody ->
     compile_equiv qbody;
     equiv_lam _ _ f (compile qbody);
@@ -51,6 +48,23 @@ let rec compile_equiv #g #a (#s:fs_oexp g a) (qs:exp_quotation g s)
       norm [delta_only [`%compile]; zeta;iota];
       rewrite_eqs_from_context ();
       assumption ())
+  | QFalse -> equiv_false g
+  | QTrue -> equiv_true g
+  | QIf #_ #_ #c qc #t qt #e qe ->
+    compile_equiv qc;
+    compile_equiv qt;
+    compile_equiv qe;
+    equiv_if c t e (compile qc) (compile qt) (compile qe)
+  | QMkpair #_ #a1 #a2 #s1 #s2 q1 q2 ->
+    compile_equiv q1;
+    compile_equiv q2;
+    equiv_pair s1 s2 (compile q1) (compile q2)
+  | QFst #_ #_ #_ #p qp ->
+    compile_equiv qp;
+    equiv_pair_fst_app p (compile qp)
+  | QSnd #_ #_ #_ #p qp ->
+    compile_equiv qp;
+    equiv_pair_snd_app p (compile qp)
 
 let compile_closed_equiv (#a:qType) (#s:get_Type a) (qs:exp_quotation #a empty (fun _ -> s))
   : Lemma (ensures (a ⦂ (s, compile_closed qs))) =
